projectVampire/dafny/storage.dfy
@@ -1,8 +1,418 @@
-#include blood.dfy
-#include transportationManager.dfy
-#include insertionSort.dfy
+// state:
+// unsafe = -1
+// unverified = 0
+// verified = 1
+// storage = 2
+// dispatch = 3
+// delivered = 4
 
-class storage {
+
+// state:
+// unsafe = -1
+// unverified = 0
+// verified = 1
+// storage = 2
+// dispatched = 3
+// delivered = 4
+
+
+datatype Blood_types = O | A | B | AB
+datatype blood_state = unsafe | unverified | verified | storage | dispatched | delivered
+
+
+// Magic number in expiry time 86400(seconds in day) * 7 =  604800
+class Blood{
+    var state: blood_state;
+    var collection_time: int; //Seconds since Unix Epoch
+    var expiry_time:int
+    var blood_type: Blood_types;
+    var rhesus: bool;
+
+    predicate method Valid()
+    reads this
+    {state== unsafe || state==unverified || state==verified || state==storage || state==dispatched || state==delivered}
+
+    predicate method expired(curr_time:int)
+    reads this
+    {curr_time>expiry_time}
+
+    predicate method safe(curr_time:int)
+    reads this
+    {(state==unverified || state==verified || state==storage || state==dispatched || state==delivered) && !expired(curr_time)}
+
+    method getExpiryTime() returns (expiry : int)
+    // reads this;
+    ensures expiry == expiry_time
+    {
+        expiry := expiry_time;
+        return;
+    }
+
+    method reject_blood()
+    modifies this;
+    ensures state == unsafe
+    ensures Valid()
+    {
+        state := unsafe;
+    }
+
+    method get_blood_type() returns (b_type:Blood_types,rh:bool)
+    ensures b_type==blood_type
+    ensures rh==rhesus
+    {
+        b_type := blood_type;
+        rh := rhesus;
+    }
+
+    method get_state() returns (bl_state:blood_state)
+    ensures bl_state == state
+    {
+        bl_state := state;
+    }
+
+    constructor (secondsin:int)
+    modifies this
+    requires secondsin>=0
+    ensures collection_time>=0 && collection_time==secondsin
+    ensures state == unverified;
+    {
+        collection_time := secondsin;
+        expiry_time:=secondsin + 604800;
+        state := unverified;
+    }
+
+    method verify_blood(curr_time:int,accepted:bool,determined_type:Blood_types,rhesus_in:bool)
+    modifies this;
+    requires state==unverified
+    requires Valid()
+    ensures if (safe(curr_time) && accepted) then state == verified else state==unsafe
+    ensures blood_type==determined_type
+    ensures rhesus == rhesus_in
+    ensures Valid()
+    {
+        if safe(curr_time) && accepted {
+            state:=verified;
+        } else {
+            state:=unsafe;
+        }
+
+        blood_type:=determined_type;
+        rhesus:=rhesus_in;
+    }
+
+    method store_blood(curr_time:int)
+    modifies this
+    requires Valid()
+    requires state==verified;
+    ensures if safe(curr_time) then state == storage else state==unsafe;
+    ensures Valid()
+    {
+        if safe(curr_time) {
+            state:=storage;
+        } else {
+            state:=unsafe;
+        }  
+    }
+
+    method dispatch_blood(curr_time:int)
+    modifies this
+    requires Valid()
+    requires state==storage;
+    ensures if safe(curr_time) then state == dispatched else state==unsafe;
+    ensures Valid()
+    {
+        if safe(curr_time) {
+            state:=dispatched;
+        } else {
+            state:=unsafe;
+        }         
+    }
+
+    method deliver_blood(curr_time:int)
+    modifies this
+    requires Valid()
+    requires state==dispatched;
+    ensures if safe(curr_time) then state ==delivered else state==unsafe;
+    ensures Valid()
+    {
+        if safe(curr_time) {
+            state:=delivered;
+        } else {
+            state:=unsafe;
+        }           
+    }
+
+    method reject()
+    modifies this
+    ensures state ==unsafe;
+    ensures Valid()
+    {state:=unsafe;}
+}
+
+/////////////////////////////////////////////////////////////////////////////////////////////
+
+//#include blood.dfy
+
+class transportationManager {
+	
+	var locale: int; // give each location an int value?
+	var destinations: array<int>; //:= new int[10]; // routes to destinations
+	var toSend: array<Blood>;// := new Blood[10]; // may need to have another array that matches the blood destinations to each index or create a class that can hold blood and its dest
+    	var toDest: array<int>;// := new int[10]; // routes (match with toSend array)
+
+    	
+
+	// Blood always has a destination, ie every blood in array is matched by a route
+	predicate method Valid()
+	//requires toDest != null;
+	//requires toSend != null
+	reads this;
+	//reads toDest[0],toDest[1], toDest[2],toDest[3],toDest[4],toDest[5],toDest[6],toDest[7],toDest[8],toDest[9];
+	requires toDest != null;
+	requires toSend != null;
+	{
+        	//forall x,y:: 0 <= x < toDest.Length && 0 <= y < toSend.Length && x == y ==> toDest[x]!=-1 && toSend[y] != null
+    		toDest !=null && toSend != null
+	}
+
+
+	method Init(src: int)
+	modifies this;
+	modifies toDest;
+	modifies toSend;
+	modifies `locale;
+	requires src >= 0
+	ensures toDest != null;
+	ensures toSend != null;
+	ensures Valid()
+	{
+		locale := src;
+		toDest := new int[10];
+		toSend := new Blood[10];
+		//var i := 0;
+		//assert toSend != null;
+		//while (i < toSend.Length) 
+		//invariant 0 <= i < toSend.Length
+		//{	
+		//	toSend[i] := null;
+		//	i := i + 1;
+		//}
+		//i := 0;
+		//while (i < toDest.Length)
+		//invariant 0 <= i < toDest.Length
+		//{
+		//	toDest[i] := -1;
+		//	i := i + 1;
+		//}
+	}
+
+		
+	method receive(bld:Blood, dst:int)
+	modifies this.toDest
+	modifies this.toSend 
+	requires toSend != null
+	requires toDest != null
+	requires forall x :: 0 <= x < toSend.Length ==> bld != toSend[x] // blood is not already in toSend
+	requires bld != null;
+	requires toSend.Length == toDest.Length
+	requires dst >= 0;
+	requires Valid(); ensures Valid();
+	//ensures forall x, y:: 0 <= x < toSend.Length && 0 <= y < toDest.Length && x == y ==> toSend[x] == bld && toDest[y] == dst -> need to fix
+	{
+       		var cDest := -1;
+		if (dst == -1) {
+			cDest := 3; // need to grab the dest that system spits out
+		} else {
+			cDest := -1;
+		}
+		//var index := 0;
+		//var i := 0;
+		//while (index < toSend.Length) 
+		//invariant 0 <= i <= toSend.Length
+		//{
+		//	if (toSend[i] == null) {
+		//		index := i;
+		//		i := toSend.Length -1;		
+		//	}
+		//	i :=  i + 1;
+		//}
+		//toSend[i] := bld;
+		//toDest[i] := cDest;
+
+		var i := 0;
+		var j := 0;
+		while (i < toSend.Length && j < toDest.Length)
+		invariant 0 <= i <= toSend.Length
+		invariant 0 <= j <= toDest.Length
+		//invariant forall x,y :: 0 <= x < toSend.Length && 0 <= y < toDest.Length && toDest[y] == cDest && toSend[x] == bld ==> (x==y) -> need to fix
+		//invariant forall x :: 0 <= x < (j-1) ==> toDest[x] != 0
+		//invariant forall x, y :: 0 <= x < i && 0 <= y < j && x == y ==> toSend[x] == bl
+		invariant i == j
+		{
+			if (toSend[i] == null && toDest[j] == 0) {
+				toSend[i] := bld;
+				toDest[j] := cDest;
+				//i := toSend.Length -1;
+				//j := toDest.Length -1;
+			}
+			i := i + 1;
+			j := j + 1;
+		}
+    	}
+
+
+	method dispatchBlood()
+	modifies toSend;
+	modifies toDest;
+	requires toSend != null;
+	requires toDest != null;
+	requires exists x :: 0 <= x < toSend.Length && toSend[x] != null // blood is to be sent
+	requires Valid();ensures Valid();
+    	ensures forall x, y:: 0 <= x < toSend.Length && 0 <= y < toDest.Length  && x == y ==> (toSend[x] == null && toDest[y] == 0) // toSend and toRoute are empty
+	{
+		var i := 0;
+		var j := 0;
+		while (i < toSend.Length && j < toDest.Length)
+		invariant 0 <= i <= toSend.Length
+		invariant 0 <= j <= toDest.Length
+		invariant forall x :: 0 <= x < i ==> toSend[x] == null
+		invariant forall x :: 0 <= x < j ==> toDest[x] == 0
+		invariant i == j
+		{
+			toDest[j] := 0;
+			toSend[i] := null;
+			i := i + 1;
+			j := j + 1;
+		}
+		
+    	}
+    
+}
+
+/////////////////////////////////////////////////////////////////////////////////////////////
+
+predicate Sorted(arr: array<int>, start:int, end:int)
+requires arr != null;
+requires 0<=start<arr.Length;
+requires end <= arr.Length;
+//requires forall x :: 0 <= x < arr.Length ==> arr[x] != null;
+reads arr;
+{
+    forall i, j :: start <= i < j < end ==> arr[i] <= arr[j]
+}
+
+
+
+// Expiry time and values in two arrays match
+predicate Matching(arr1: array<int>, arr2: array<Blood>)
+requires arr1 != null;
+requires arr2 != null;
+requires arr1.Length == arr2.Length;
+reads arr1;
+reads arr2;
+reads arr2[..];
+{
+	forall i :: 0 <= i < arr1.Length && arr2[i] != null ==> arr2[i].expiry_time == arr1[i]
+}
+
+
+//method bloodSort(toSort: array<Blood>, sortedArray: array<int>) returns (sortedBlood: array<Blood>)
+//modifies toSort;
+//requires toSort != null;
+//requires sortedArray != null;
+//requires forall x :: exists y :: 0 <= x < toSort.Length && 0 <= y < sortedArray.Length && toSort[x] != null && toSort[x].expiry_time == sortedArray[y] // requires mapping from sorted to toSort
+//requires toSort.Length == sortedArray.Length;
+//ensures sortedBlood != null;
+//ensures toSort.Length == sortedBlood.Length;
+//ensures forall x :: 0 <= x < sortedBlood.Length && sortedBlood[x] != null ==> sortedBlood[x].expiry_time == sortedArray[x]; // a mapping between sorted array an blood expiry
+//{
+//	var x := 0;
+//	var y := 0;
+//	sortedBlood := new Blood[toSort.Length]; 
+//	while x < toSort.Length 
+//	invariant 0 <= x <= toSort.Length
+//	//invariant forall i :: 0 <= i < x ==> sortedBlood[i] != null
+//	//invariant forall i :: 0 <= i < x  && sortedBlood[i] != null==> sortedBlood[i].expiry_time == sortedArray[i]
+//	{
+//		 
+//		y := 0;
+//		while y < toSort.Length 
+//			invariant 0 <= y <= toSort.Length
+//			//invariant forall i :: 0 <= i < y && toSort[i] != null && sortedBlood[i] != null && sortedBlood[i] == toSort[x] ==> i == y
+//			//invariant exists i :: 0 <= i < (y-1) && toSort[i] != null && toSort[i].expiry_time == sortedArray[i]
+//			{
+//			if (toSort[y] != null && sortedArray[x] == toSort[y].expiry_time) {
+//				sortedBlood[x] := toSort[x];
+//				toSort[y] := null; // so we don't capture this object again
+//			}
+//			y := y + 1;
+//		}	 
+//		x := x + 1;
+//	}
+//}
+
+
+
+
+
+
+
+
+method insertionSort(toSort: array<int>, toMatch: array<Blood>)
+requires toSort != null;
+requires toMatch != null;
+requires toSort.Length == toMatch.Length;
+//requires forall x :: 0 <= x < toSort.Length ==> toSort[x] != null
+requires forall x,y ::0 <= x < toSort.Length && 0 <= y < toMatch.Length && x == y  && toMatch[y] != null ==> toMatch[y].expiry_time == toSort[x];
+
+requires toSort.Length > 1;
+ensures Sorted(toSort,0,toSort.Length-1);
+ensures multiset(toSort[..]) == multiset(old(toSort[..]));
+ensures forall x, y :: 0 <= x < toSort.Length && 0 <= y < toMatch.Length && x == y && toMatch[y] != null ==> toMatch[y].expiry_time == toSort[x];
+modifies toSort;
+modifies toMatch;
+{
+    var start := 1;
+    while (start < toSort.Length)
+    invariant 1 <= start <= toSort.Length;
+    invariant Sorted(toSort, 0, start); // array is sorted up to start
+    invariant multiset(toSort[..]) == multiset(old(toSort[..])); // keep array the same
+    invariant multiset(toMatch[..]) == multiset(old(toMatch[..]));
+    invariant forall x, y :: 0 <= x < toMatch.Length && 0 <= toSort.Length && x == y && toMatch[x] != null ==> toSort[y] == toMatch[x].expiry_time;
+    //invariant Matching(toSort, toMatch);
+    //invariant forall x :: 0 <= x < toSort.Length ==> toSort[x] != null
+    //invariant forall x :: 0 <= x < toSort.Length 
+    {
+        var end := start;
+        while (end >= 1 && toSort[end-1] > toSort[end])
+        invariant 0 <= end <= start; // end is within limits
+        invariant multiset(toSort[..]) == multiset(old(toSort[..])); // array stays the same
+	invariant multiset(toMatch[..]) == multiset(old(toMatch[..]));
+	//invariant Matching(toSort, toMatch);
+	//invariant forall i :: 0 <= i < toSort.Length ==> toSort[i] != null;
+        invariant forall i, j :: (0 <= i <= j <= start && j != end) ==> toSort[i] <= toSort[j]; // all values less than start are sorted
+        //invariant forall i :: (0 <= i <= start && i != end && toMatch[i] != null) ==> toSort[i] == toMatch[i].expiry_time;
+        invariant forall x, y :: 0 <= x < toMatch.Length && 0 <= toSort.Length && x == y && toMatch[x] != null ==> toSort[y] == toMatch[x].expiry_time;
+	{
+           	var temp := toSort[end-1];
+           	toSort[end-1] := toSort[end];
+            	toSort[end] := temp;
+		
+	    	var temp2 := toMatch[end-1];
+	    	toMatch[end-1] := toMatch[end];
+	    	toMatch[end] := temp2;
+		
+		end := end -1;
+		
+        }
+        start := start + 1;
+    }
+}
+
+
+/////////////////////////////////////////////////////////////////////////////////////////////
+
+class Storage {
 
     // Index for bloodStorage
     // AP_blood = 0
@@ -18,147 +428,191 @@ class storage {
     var name: string;
     var Xcoordinate: int;
     var Ycoordinate: int;
-    var bloodStorage: array<array<blood>>;
+    var bloodStorage: array<array<Blood>>;
     var transManager: transportationManager;
-    var node: Node
+
+    predicate eightBloodTypes(a: array<array<Blood>>)
+    requires a != null
+    reads a
+    {
+        a.Length == 8
+    }
 
     // Constructor
-    constructor (n: string, x: int, y: int) {
+    constructor (n: string, x: int, y: int)
+    modifies this
+    ensures name == n && Xcoordinate == x && Ycoordinate == y && transManager == null
+    ensures bloodStorage != null && eightBloodTypes(bloodStorage)
+    ensures storageInitialised(bloodStorage)
+    {
         name := n;
         Xcoordinate := x;
         Ycoordinate := y;
         bloodStorage := new array[8];
-        i := 0;
-        while (i < bloodStorage.length) {
-            bloodStorage[i] := new blood[100];
-            i := i + 1;
-        }
+        initBloodStorage(bloodStorage);
         transManager := null;
-        node := null;
     }
 
-    method setNode(n: Node) {
-        node := n;
+    predicate storageInitialised(a: array<array<Blood>>)
+    requires a != null
+    reads a
+    {
+        forall k :: 0 <= k < a.Length ==> a[k] != null
+    }
+
+    // Initialises bloodStorage with 8 arrays to store each type of blood
+    method initBloodStorage(bloodStorage: array<array<Blood>>)
+    requires bloodStorage != null
+    modifies bloodStorage
+    ensures storageInitialised(bloodStorage)
+    {
+        var len := bloodStorage.Length;
+        var i := 0;
+        while i < len
+        decreases len - i
+        invariant i - 1 < len
+        invariant forall k :: 0 <= k < i <= len ==> bloodStorage[k] != null
+        {
+            bloodStorage[i] := new Blood[10];
+            i := i + 1;
+        }
     }
 
     // Adds a transportation manager
-    method setTransportationManager(manager: transportationManager) {
+    method setTransportationManager(manager: transportationManager)
+    modifies this
+    ensures transManager == manager
+    {
         transManager := manager;
     }
 
+    // ISSUE: For some reason the error is that bloodStorage might be null,
+    //        despite my requires bloodStorage != null
+    
     // Stores blood and sorts according to expiry
-    method storeBlood(b: blood) {
-        index := findIndex(blood.blood_type, blood.rhesus);
-        var prevSize := bloodStorage[index].length;
-        var newArray := new array[prevSize+1];
+    method storeBlood(b: Blood)
+    requires b != null
+    requires bloodStorage != null && eightBloodTypes(bloodStorage)
+    requires storageInitialised(bloodStorage)
+    modifies bloodStorage
+    {
+        var index := findIndex(b.blood_type, b.rhesus);
+        var prevSize := bloodStorage[index].Length;
+        
+        var newArray := new Blood[prevSize+1];
         var i := 0;
-        while (i < prevSize) {
-            newArray[i] := bloodStorage[index][i];
+        while i < prevSize
+        decreases prevSize - i
+        invariant i - 1 < prevSize
+        //invariant forall k :: 0 <= k < i <= prevSize ==> newArray[k] == bloodStorage[index][k]
+        {
+            //newArray[i] := bloodStorage[index][i];
             i := i + 1;
         }
-        newArray[prevSize] := blood;
+        
+        /*
+        newArray[prevSize] := b;
         bloodStorage[index] := newArray;
 
         // Generate list of blood times
         var valuearray := new array[bloodStorage[index].length];
         i := 0;
-        while (i < bloodStorage[index].length) {
+        while (i < bloodStorage[index].Length) {
             valuearray[i] := bloodStorage[index][i].getExpiryTime();
         }
 
         insertionSort(valuearray, bloodStorage[index]);
+        */
     }
 
-    // Discard expired blood
-    method discardBlood(currTime: int) {
-        i := 0;
-        while (i < bloodStorage.length) {
-            numToDiscard := 0;
-            j := 0;
-            while (j < bloodStorage[i].length) {
-                if (currTime - bloodStorage[i][j].expiry_time < 60*60*24*2) {
-                    numToDiscard := numToDiscard + 1;
-                }
-                j := j + 1;
-            }
-            removeN(i, numToDiscard);
-            i := i + 1;
-        }
-    }
-
-    // Gets appropriate blood packet from storage and notifies transport to send it to destination
-    method serviceRequest(t: blood_type, rh: bool, dest: string) {
-        index := findIndex(t, rh);
-        blood := pop(index);
-        if (blood == null) {
-            print("No blood of requested type available");
-        }
-        else {
-            notifyTransport(blood, dest);
-        }
-    }
+    // ISSUE: There are extra requires clauses in transportationManager's receive()
+    //        that storage cannot supply. Storage can only require the below successfully,
+    //        is it possible to change receive() so that it can be called from here?
 
     // Gives blood to transport so that they can prepare to dispatch it to the destination
-    method notifyTransport(b: blood, dest: string) {
-        transManager.receive(b, dest);
-        transManager.dispatchBlood();
+    method notifyTransport(b: Blood, dest: int)
+    requires b != null
+    requires transManager != null
+    {
+        //transManager.receive(b, dest);
+        //transManager.dispatchBlood();
     }
+
+    // ISSUE: Verification not completed, need ensures clause
 
     // Helper: Remove head of array and return it
-    method pop(index: int) returns (b: blood) {
-        a := bloodStorage[index];
-        if (a.length < 1) {
-            return null;
+    method pop(index: int) returns (b: Blood)
+    requires 0 <= index <= 7
+    requires bloodStorage != null && storageInitialised(bloodStorage)
+    requires eightBloodTypes(bloodStorage)
+    modifies bloodStorage
+    {
+        var a := bloodStorage[index];
+
+        if (a.Length < 1) {
+            b := null;
         }
-        b := a[0];
-        newArray := new array[a.length-1];
-        i := 0;
-        while (i + 1 < a.length) {
-            newArray[i] := a[i + 1];
-            i := i + 1;
+        else {
+            b := a[0];
+            var newArray := new Blood[a.Length-1];
+            var i := 0;
+            while i + 1 < a.Length
+            decreases a.Length - (i + 1)
+            invariant i < a.Length
+            {
+                newArray[i] := a[i + 1];
+                i := i + 1;
+            }
+            bloodStorage[index] := newArray;
         }
-        bloodStorage[index] := newArray;
     }
 
-    // Helper: Remove n elements from head of array
-    method removeN(index: int, numToDiscard: int) {
-        a := bloodStorage[index];
-        newArray := new array[a.length-numToDiscard];
-        i := 0;
-        while (i + numToDiscard < a.length) {
-            newArray[i] := a[i + numToDiscard];
-        }
-        bloodStorage[index] := newArray;
+
+
+    // Ensures that a certain blood type and rhesus corresponds to the correct index
+    predicate correctIndex(t: Blood_types, rh: bool, index: int)
+    reads this
+    {
+        (t == A && rh ==> index == 0) &&
+        (t == A && !rh ==> index == 1) &&
+        (t == B && rh ==> index == 2) &&
+        (t == B && !rh ==> index == 3) &&
+        (t == AB && rh ==> index == 4) &&
+        (t == AB && !rh ==> index == 5) &&
+        (t == O && rh ==> index == 6) &&
+        (t == O && !rh ==> index == 7) &&
+        (0 <= index <= 7)
     }
 
     // Helper: Returns the index that is storing the required blood type
-    method findIndex(t: blood_type, rh: bool) returns (index: int) {
-        if (t == O & rh) {
+    method findIndex(t: Blood_types, rh: bool) returns (index: int)
+    ensures correctIndex(t, rh, index)
+    {
+        if (t == A && rh) {
             index := 0;
         }
-        else if (t == A & rh) {
+        else if (t == A && !rh) {
             index := 1;
         }
-        else if (t == B & rh) {
+        else if (t == B && rh) {
             index := 2;
         }
-        else if (t == AB & rh) {
+        else if (t == B && !rh) {
             index := 3;
         }
-        else if (t == O & !rh) {
+        else if (t == AB && rh) {
             index := 4;
         }
-        else if (t == A & !rh) {
+        else if (t == AB && !rh) {
             index := 5;
         }
-        else if (t == B & !rh) {
+        else if (t == O && rh) {
             index := 6;
         }
-        else if (t == AB & !rh) {
+        else if (t == O && !rh) {
             index := 7;
         }
     }
 
-
-
 }
+
